UnsafeAccess.v
@@ -1,0 +1,366 @@
+From Coq Require Import Logic.Classical_Prop.
+From Coq Require Import Arith.Arith.
+From Coq Require Import Lia.
+
+From Elo Require Import Util.
+From Elo Require Import Array.
+From Elo Require Import Map.
+From Elo Require Import Core.
+From Elo Require Import Contains.
+From Elo Require Import Access.
+From Elo Require Import ValidAccesses.
+From Elo Require Import References.
+From Elo Require Import AccessProp.
+
+Inductive UnsafeAccess (m : mem) : tm -> addr -> Prop :=
+  | uacc_mem : forall ad ad' T,
+    ad <> ad' ->
+    UnsafeAccess m m[ad'] ad ->
+    UnsafeAccess m <{ &ad' :: &T }> ad
+
+  | uacc_ref : forall ad T,
+    UnsafeAccess m <{ &ad :: &T }> ad
+
+  | uacc_new : forall T t ad,
+    UnsafeAccess m t ad ->
+    UnsafeAccess m <{ new T t }> ad
+
+  | uacc_load : forall t ad,
+    UnsafeAccess m t ad ->
+    UnsafeAccess m <{ *t }> ad
+
+  | uacc_asg1 : forall t1 t2 ad,
+    UnsafeAccess m t1 ad ->
+    UnsafeAccess m <{ t1 = t2 }> ad
+
+  | uacc_asg2 : forall t1 t2 ad,
+    UnsafeAccess m t2 ad ->
+    UnsafeAccess m <{ t1 = t2 }> ad
+
+  | uacc_fun : forall x Tx t ad,
+    UnsafeAccess m t ad ->
+    UnsafeAccess m <{ fn x Tx --> t }> ad
+
+  | uacc_call1 : forall t1 t2 ad,
+    UnsafeAccess m t1 ad ->
+    UnsafeAccess m <{ call t1 t2 }> ad
+
+  | uacc_call2 : forall t1 t2 ad,
+    UnsafeAccess m t2 ad ->
+    UnsafeAccess m <{ call t1 t2 }> ad
+
+  | uacc_seq1 : forall t1 t2 ad,
+    UnsafeAccess m t1 ad ->
+    UnsafeAccess m <{ t1; t2 }> ad
+
+  | uacc_seq2 : forall t1 t2 ad,
+    UnsafeAccess m t2 ad ->
+    UnsafeAccess m <{ t1; t2 }> ad
+  .
+
+Ltac inversion_uacc :=
+  match goal with
+  | H : UnsafeAccess _ <{ unit         }> _ |- _ => inversion H; subst
+  | H : UnsafeAccess _ <{ N _          }> _ |- _ => inversion H; subst
+  | H : UnsafeAccess _ <{ & _ :: _     }> _ |- _ => inversion H; subst
+  | H : UnsafeAccess _ <{ new _ _      }> _ |- _ => inversion H; subst
+  | H : UnsafeAccess _ <{ * _          }> _ |- _ => inversion H; subst
+  | H : UnsafeAccess _ <{ _ = _        }> _ |- _ => inversion H; subst
+  | H : UnsafeAccess _ <{ var _        }> _ |- _ => inversion H; subst
+  | H : UnsafeAccess _ <{ fn _ _ --> _ }> _ |- _ => inversion H; subst
+  | H : UnsafeAccess _ <{ call _ _     }> _ |- _ => inversion H; subst
+  | H : UnsafeAccess _ <{ _ ; _        }> _ |- _ => inversion H; subst
+  | H : UnsafeAccess _ <{ spawn _      }> _ |- _ => inversion H; subst
+  end.
+
+Ltac inversion_clear_uacc :=
+  match goal with
+  | H : UnsafeAccess _ <{ unit         }> _ |- _ => inversion_subst_clear H
+  | H : UnsafeAccess _ <{ N _          }> _ |- _ => inversion_subst_clear H
+  | H : UnsafeAccess _ <{ & _ :: _     }> _ |- _ => inversion_subst_clear H
+  | H : UnsafeAccess _ <{ new _ _      }> _ |- _ => inversion_subst_clear H
+  | H : UnsafeAccess _ <{ * _          }> _ |- _ => inversion_subst_clear H
+  | H : UnsafeAccess _ <{ _ = _        }> _ |- _ => inversion_subst_clear H
+  | H : UnsafeAccess _ <{ var _        }> _ |- _ => inversion_subst_clear H
+  | H : UnsafeAccess _ <{ fn _ _ --> _ }> _ |- _ => inversion_subst_clear H
+  | H : UnsafeAccess _ <{ call _ _     }> _ |- _ => inversion_subst_clear H
+  | H : UnsafeAccess _ <{ _ ; _        }> _ |- _ => inversion_subst_clear H
+  | H : UnsafeAccess _ <{ spawn _      }> _ |- _ => inversion_subst_clear H
+  end.
+
+Lemma uacc_dec : forall m t ad,
+  Decidable.decidable (UnsafeAccess m t ad).
+Proof. eauto using classic_decidable. Qed.
+
+(* ------------------------------------------------------------------------- *)
+(* negation                                                                  *)
+(* ------------------------------------------------------------------------- *)
+
+Local Ltac solve_nuacc :=
+  intros; try (split; intros); eauto using UnsafeAccess.
+
+Lemma nuacc_new : forall m t ad T,
+  ~ UnsafeAccess m <{ new T t }> ad ->
+  ~ UnsafeAccess m t ad.
+Proof. solve_nuacc. Qed.
+
+Lemma nuacc_load : forall m t ad,
+  ~ UnsafeAccess m <{ *t }> ad ->
+  ~ UnsafeAccess m t ad.
+Proof. solve_nuacc. Qed.
+
+Lemma nuacc_asg : forall m t1 t2 ad,
+  ~ UnsafeAccess m <{ t1 = t2 }> ad ->
+  ~ UnsafeAccess m t1 ad /\ ~ UnsafeAccess m t2 ad.
+Proof. solve_nuacc. Qed.
+
+Lemma nuacc_call : forall m t1 t2 ad,
+  ~ UnsafeAccess m <{ call t1 t2 }> ad ->
+  ~ UnsafeAccess m t1 ad /\ ~ UnsafeAccess m t2 ad.
+Proof. solve_nuacc. Qed.
+
+Lemma nuacc_seq : forall m t1 t2 ad,
+  ~ UnsafeAccess m <{ t1; t2 }> ad ->
+  ~ UnsafeAccess m t1 ad /\ ~ UnsafeAccess m t2 ad.
+Proof. solve_nuacc. Qed.
+
+Ltac inversion_nuacc :=
+  match goal with
+  | H: ~ UnsafeAccess _ <{ new _ _  }> _ |- _ => eapply nuacc_new  in H
+  | H: ~ UnsafeAccess _ <{ * _      }> _ |- _ => eapply nuacc_load in H
+  | H: ~ UnsafeAccess _ <{ _ = _    }> _ |- _ => eapply nuacc_asg  in H as [? ?]
+  | H: ~ UnsafeAccess _ <{ call _ _ }> _ |- _ => eapply nuacc_call in H as [? ?]
+  | H: ~ UnsafeAccess _ <{ _ ; _    }> _ |- _ => eapply nuacc_seq  in H as [? ?]
+  end.
+
+(* ------------------------------------------------------------------------- *)
+(* core properties                                                           *)
+(* ------------------------------------------------------------------------- *)
+
+Theorem nuacc_refI : forall m ad v T,
+  value v ->
+  empty |-- v is (TY_Immut T) ->
+  ~ UnsafeAccess m v ad.
+Proof.
+  intros * Hval Htype Huacc. destruct Hval;
+  inversion_type; inversion_uacc; eauto using UnsafeAccess.
+Qed.
+
+Theorem uacc_soundness : forall m m' t t' ad eff T,
+  ad < length m ->
+  empty |-- t is T ->
+  ~ UnsafeAccess m t ad ->
+  m / t ==[eff]==> m' / t' ->
+  m[ad] = m'[ad].
+Proof.
+  intros * ? ? Hnuacc ?. rename ad into ad'. inversion_mstep; trivial.
+  - decompose sum (lt_eq_lt_dec ad' (length m)); subst;
+    simpl_array; trivial. lia.
+  - decompose sum (lt_eq_lt_dec ad' ad); subst; simpl_array; trivial.
+    generalize dependent T. induction_step; intros;
+    inversion_nuacc; inversion_type; eauto using UnsafeAccess.
+    inversion_type. exfalso. eauto using UnsafeAccess.
+Qed.
+
+Lemma uacc_then_acc : forall m t ad,
+  UnsafeAccess m t ad ->
+  access m t ad.
+Proof.
+  intros * Huacc. induction Huacc; eauto using access.
+Qed.
+
+(* ------------------------------------------------------------------------- *)
+(* safe memory sharing                                                       *)
+(* ------------------------------------------------------------------------- *)
+
+Local Definition safe_memory_sharing m ths := forall tid1 tid2 ad,
+  tid1 <> tid2 ->
+  access m ths[tid1] ad ->
+  access m ths[tid2] ad ->
+  ~ UnsafeAccess m ths[tid1] ad.
+
+Local Lemma length_tid : forall m m' t' ths tid eff,
+  m / ths[tid] ==[eff]==> m' / t' ->
+  tid < length ths.
+Proof.
+  intros * Hmstep.
+  decompose sum (lt_eq_lt_dec tid (length ths)); subst; trivial;
+  rewrite (get_default TM_Unit) in Hmstep; try lia;
+  inversion_mstep; inversion_step.
+Qed.
+
+Lemma write_then_uacc : forall m t t' ad v T,
+  empty |-- t is T ->
+  t --[EF_Write ad v]--> t' ->
+  UnsafeAccess m t ad.
+Proof.
+  intros * ? ?. generalize dependent T.
+  induction_step; intros * ?;
+  inversion_type; eauto using UnsafeAccess.
+  inversion_type. eauto using UnsafeAccess.
+Qed.
+
+Local Lemma mstep_write_sms_preservation : forall m m' ths t' tid ad v,
+  forall_threads ths (fun t => exists T, empty |-- t is T) ->
+  safe_memory_sharing m ths ->
+  m / ths[tid] ==[EF_Write ad v]==> m' / t' ->
+  safe_memory_sharing m' ths[tid <- t'].
+Proof.
+  intros * Htype Hsms Hmstep tid1 tid2 ad' Hneq Hacc1W Hacc2W.
+  specialize (Hsms _ _ ad' Hneq) as Hsms1.
+  specialize (Hsms _ _ ad' (not_eq_sym Hneq)) as Hsms2.
+  assert (Hlen : tid < length ths) by eauto using length_tid.
+  inversion Hmstep; subst.
+  destruct (Nat.eq_dec tid tid1), (Nat.eq_dec tid tid2); subst; try lia;
+  do 3 simpl_array.
+  - intros Huacc.
+    destruct (access_dec m ths[tid2] ad) as [Hacc2 | Hnacc2].
+    + assert (Hacc1 : access m ths[tid1] ad)
+        by eauto using mstep_write_requires_acc.
+      destruct (Htype tid1) as [T1 Htype1].
+      specialize (Hsms _ _ _ Hneq Hacc1 Hacc2) as ?.
+      eauto using write_then_uacc.
+    + assert (Hacc1' : access m ths[tid1] ad')
+        by eauto using mstep_write_inherits_acc.
+      assert (Hacc2' : access m ths[tid2] ad')
+        by eauto using mem_set_inherits_acc2.
+      do 4 auto_specialize.
+      eapply Hsms1.
+Abort.
+
+(* ------------------------------------------------------------------------- *)
+(* other properties                                                          *)
+(* ------------------------------------------------------------------------- *)
+
+Lemma todo1 : forall m t t' ad v,
+  t --[EF_Write ad v]--> t' ->
+  access m[ad <- v] t ad.
+Proof.
+  intros. induction_step; eauto using access.
+Qed.
+
+Lemma mem_set_inherits_uacc1 : forall m t ad ad' v,
+  ~ access m t ad' ->
+  UnsafeAccess m[ad' <- v] t ad ->
+  UnsafeAccess m t ad.
+Proof.
+  intros * Hnacc Huacc. remember (m[ad' <- v]) as m'.
+  induction Huacc; inversion_subst_clear Heqm'; inversion_not_access Hnacc;
+  eauto using UnsafeAccess.
+  do 2 simpl_array. eauto using UnsafeAccess.
+Qed.
+
+Lemma mem_set_inherits_uacc2 : forall m t ad ad' v,
+  ~ access m v ad ->
+  UnsafeAccess m[ad' <- v] t ad ->
+  UnsafeAccess m t ad.
+Proof.
+  intros * Hnacc Huacc. remember (m[ad' <- v]) as m'.
+  induction Huacc; try rename IHHuacc into IH;
+  inversion_subst_clear Heqm'; eauto using UnsafeAccess.
+  match goal with _ : _ <> ?ad |- _ => rename ad into ad'' end.
+  destruct (Nat.eq_dec ad' ad''); subst;
+  try solve [do 2 simpl_array; eauto using UnsafeAccess].
+  destruct (Nat.eq_dec ad'' ad); subst; eauto using UnsafeAccess.
+  auto_specialize. contradict Hnacc.
+  rewrite (get_set_eq TM_Unit) in IH; eauto using uacc_then_acc.
+  eapply not_le. intros Hlen. do 3 simpl_array. 
+  eapply le_lt_or_eq in Hlen as [? | ?]; subst;
+  do 2 simpl_array; inversion_uacc.
+Qed.
+
+Local Lemma simpl_uacc : forall m ad ad' v,
+  UnsafeAccess m[ad' <- v] m[ad' <- v][ad'] ad ->
+  ad' < length m.
+Proof.
+  assert (ge_iff_le : forall m n, m >= n <-> n <= m)
+    by (intros; split; destruct n; eauto).
+  intros * H. eapply not_ge. rewrite ge_iff_le. intros ?.
+  rewrite (get_set_invalid TM_Unit) in H; trivial. inversion H.
+Qed.
+
+Lemma mem_set_preserves_nuacc : forall m t ad ad' v,
+  ~ UnsafeAccess m v ad ->
+  ~ UnsafeAccess m t ad ->
+  ~ UnsafeAccess m[ad' <- v] t ad.
+Proof.
+  intros * ? ? Huacc. remember (m[ad' <- v]) as m'.
+  induction Huacc; inversion_subst_clear Heqm'; eauto using UnsafeAccess.
+  match goal with _ : _ <> ?ad |- _ => rename ad into ad'' end. 
+  destruct (Nat.eq_dec ad' ad'') as [? | Hneq]; subst;
+  try (assert (ad'' < length m) by eauto using simpl_uacc);
+  do 2 simpl_array; eauto using UnsafeAccess.
+Qed.
+
+Local Lemma todo : forall m t t' ad ad' v,
+  ~ UnsafeAccess m[ad' <- v] t' ad ->
+  t --[EF_Write ad' v]--> t' ->
+  ~ UnsafeAccess m t ad.
+Proof.
+  intros * Hnuacc Hstep Huacc. induction_step;
+  try solve [inversion_nuacc; inversion_uacc; eauto].
+  - inversion_nuacc. inversion_uacc; eauto using UnsafeAccess.
+Abort.
+
+Lemma mstep_write_inherits_uacc : forall m m' t t' ad ad' v,
+  UnsafeAccess m' t' ad ->
+  m / t ==[EF_Write ad' v]==> m' / t' ->
+  UnsafeAccess m t ad.
+Proof.
+  intros * Huacc ?. inversion_mstep. induction_step;
+  try solve [inversion_uacc; eauto using UnsafeAccess].
+  - inversion_uacc; eauto using UnsafeAccess.
+    destruct (uacc_dec m[ad' <- v] t1' ad); eauto using UnsafeAccess.
+    clear IHstep.
+    eapply uacc_asg2.
+    destruct (uacc_dec m v ad). 
+    + destruct (access_dec m t2 ad'); eauto using mem_set_inherits_uacc1.
+      admit.
+    + destruct (uacc_dec m t2 ad); trivial; exfalso.
+      contradict H3. eauto using (mem_set_preserves_nuacc _ t2).
+  - admit.
+  - admit.
+  - admit.
+  - admit.
+Abort.
+
+Lemma contains_nuacc : forall m t t' ad,
+  ~ UnsafeAccess m t ad ->
+  t contains t' ->
+  ~ UnsafeAccess m t' ad.
+Proof.
+  intros * ? Hcon ?. induction Hcon; subst; eauto;
+  inversion_nuacc; eauto.
+Qed.
+
+Lemma mstep_write_preserves_nuacc : forall m m' t t' ad ad' v,
+  ~ UnsafeAccess m t ad ->
+  m / t ==[EF_Write ad' v]==> m' / t' ->
+  ~ UnsafeAccess m' t' ad.
+Proof.
+  intros * ? ? ?. inversion_mstep. induction_step;
+  inversion_nuacc; inversion_clear_uacc; eauto using UnsafeAccess;
+  match goal with H : UnsafeAccess _ ?t _ |- _ => rename t into tx end;
+  eapply (mem_set_preserves_nuacc _ tx _ _ v);
+  eauto using step_write_contains_val, contains_nuacc.
+Qed.
+
+
+
+
+
+
+
+
+
+
+
+
+
+
+
+
+
+
+
+
